g_string_syntax.ml
@@ -5,8 +5,7 @@
 (*    //   *      This file is distributed under the terms of the      *)
 (*         *       GNU Lesser General Public License Version 2.1       *)
 (***********************************************************************)
-open Coqast
-open Ast
+
 open Pp
 open Util
 open Names
@@ -14,78 +13,60 @@ open Pcoq
 open Libnames
 open Topconstr
 open G_ascii_syntax
+open Rawterm
 
 exception Non_closed_string
 
 (* make a string term from the string s *)
 
-let cstring loc = Qualid (loc,make_qualid ["String"] "String")
-let cemptystring loc = Qualid (loc,make_qualid ["String"] "EmptyString")
+let string_module = make_dir ["String"]
+let string_path = make_path string_module (id_of_string "string")
+let glob_String  = ConstructRef ((string_path,0),1)
 
-let make_string s dloc =
-  let le = (String.length s) in
-  let rec aux n = 
-     if n = le then CRef (cemptystring dloc) else
-     CAppExpl (dloc,(None,cstring dloc),
-       [make_ascii dloc (int_of_char s.[n]); aux (n+1)])
-     in aux 0
-
-GEXTEND Gram
-  GLOBAL: Constr.operconstr;
-  Constr.operconstr: LEVEL "0" [ [ s = STRING -> make_string s loc ] ];
-END
-
-(** old ast-based pp **)
-
-open Termast
-
-let ascii_path = make_path (make_dir ["Ascii"]) (id_of_string "ascii")
-let path_of_Ascii  = ((ascii_path,0),1)
-let glob_Ascii  = ConstructRef path_of_Ascii
-
-let string_path = make_path (make_dir ["String"]) (id_of_string "string")
+let glob_string  = IndRef (string_path,0)
 let path_of_EmptyString  = ((string_path,0),1)
 let glob_EmptyString  = ConstructRef path_of_EmptyString
 let path_of_String  = ((string_path,0),2)
 let glob_String  = ConstructRef path_of_String
 
-let astAscii = ast_of_ref glob_Ascii
-let astEmptyString = ast_of_ref glob_EmptyString
-let astString = ast_of_ref glob_String
+let interp_string dloc s =
+  let le = String.length s in
+  let rec aux n = 
+     if n = le then RRef (dloc, glob_EmptyString) else
+     RApp (dloc,RRef (dloc, glob_String),
+       [interp_ascii dloc (int_of_char s.[n]); aux (n+1)])
+     in aux 0
 
-let rec ascii_of_ast p =
-  match p with
-    | Node (_,"APPLIST", (b::l)) when alpha_eq(b,astAscii) ->
-        (match alist_val l with
-          | None -> raise Non_closed_string
-          | Some l -> 
-              let v = String.make 1 (char_of_int l) in
-              if v="\"" || v="\\"   then "\\"^v else v)
-    | _ -> raise Non_closed_string
+let interp_string_pat dloc s name =
+  let le = String.length s in
+  let rec aux n = 
+     if n = le then PatCstr (dloc,path_of_EmptyString,[],name) else
+     PatCstr (dloc,path_of_String,
+       [interp_ascii_pat dloc (int_of_char s.[n]) Anonymous; aux (n+1)],name)
+     in aux 0
 
-let rec string_of_ast p =
-  match p with
-    | b when alpha_eq(b,astEmptyString) ->
-        ""
-    | Node (_,"APPLIST", [b;c;d]) when alpha_eq(b,astString) ->
-        (ascii_of_ast c)^(string_of_ast d)
-    | _ -> raise Non_closed_string
-
-let string_printer p =
+let uninterp_string r =
   try 
-    match p with
-    | Node (_,"STRING", [c;d]) -> 
-        Some (str "\"" ++ str ((ascii_of_ast c)^(string_of_ast d)) ++ str "\"")
-    | _ -> failwith "Inconsistent pretty-printer rule"
+    let b = Buffer.create 16 in
+    let rec aux = function
+    | RApp (_,RRef (_,k),[a;s]) when k = glob_String ->
+	(match uninterp_ascii a with
+	  | Some c -> Buffer.add_char b (Char.chr c); aux s
+	  | _ -> raise Non_closed_string)
+    | RRef (_,z) when z = glob_EmptyString ->
+	Some (Buffer.contents b)
+    | _ ->
+	raise Non_closed_string
+    in aux r
   with 
    Non_closed_string -> None
 
-let _ = if !Options.v7 then
-  Esyntax.declare_primitive_printer "string_printer" "string_scope" 
-    string_printer
+let _ =
+  Notation.declare_string_interpreter "string_scope"
+    (glob_string,["String"])
+    (interp_string,Some interp_string_pat)
+    ([RRef (dummy_loc,glob_String);RRef (dummy_loc,glob_EmptyString)],
+     uninterp_string, None)
 
 
-
-
-
-
+(* uninterp_string_pat *)
