Ascii_syntax.v
@@ -15,28 +15,17 @@ Declare ML Module "g_ascii_syntax".
 
 (* Parsing *)
 
-
-(*
-Grammar ascii explode :=.
-
-Grammar constr constr0 :=
-  ascii [ "@" ascii:explode($c)] -> [$c].
-*)
-
 Delimit Scope string_scope with string.
 Open Scope string_scope.
-
-(* Pretty-printing *)
-
-(* <Warning> : Syntax is discontinued *)
 
 (* Examples *)
 
 Eval compute in zero.
 Eval compute in (nat2ascii 65).
 Eval compute in (fun x : bool => Ascii x x x x x x x x).
-Eval compute in (Ascii false false false false false false false false).
-Eval compute in (Ascii true false false false false false false false).
-Eval compute in (Ascii false true false false false true false false).
-Eval compute in (Ascii false false true true true false true false).
-Eval compute in (Ascii true true true false true false false false).
+Eval compute in @@"000".
+Eval compute in @@"001".
+Eval compute in @@"""".
+Eval compute in @@"\\".
+Eval compute in @@"023".
+
