String_syntax.v
@@ -5,71 +5,13 @@ Require Export Ascii_syntax.
 
 Declare ML Module "g_string_syntax".
 
-(* Parsing and pretty-printing of strings are the usual ones
-*)
-
-(* Parsing *)
-
-(*
-Grammar sstring explode :=.
-
-Grammar constr constr0 :=
-  sstring [ sstring:explode($c)] -> [$c].
-*)
-
-(* Pretty-printing *)
-
-(* <Warning> : Syntax is discontinued *)
 (* Examples *)
 
-Eval compute in
-  (String (nat2ascii 72)
-     (String (nat2ascii 101)
-        (String (nat2ascii 108)
-           (String (nat2ascii 108) (String (nat2ascii 111) EmptyString))))).
-Eval compute in EmptyString.
-Eval compute in
-  (fun x =>
-   String x
-     (String (Ascii false false false true false true true false)
-        (String (Ascii true false true false false true true false)
-           (String (Ascii false false true true false true true false)
-              (String (Ascii false false true true false true true false)
-                 (String (Ascii true true true true false true true false)
-                    EmptyString)))))).
-Eval compute in
-  (String (Ascii false false true true true false true false) EmptyString).
-Eval compute in
-  (String (Ascii false true false false false true false false) EmptyString).
-Eval compute in
-  (let v :=
-     String (Ascii false false false true false false true false)
-       (String (Ascii true false true false false true true false)
-          (String (Ascii false false true true false true true false)
-             (String (Ascii false false true true false true true false)
-                (String (Ascii true true true true false true true false)
-                   (String
-                      (Ascii false false false false false true false false)
-                      (String
-                         (Ascii true true true false true true true false)
-                         (String
-                            (Ascii true true true true false true true false)
-                            (String
-                               (Ascii false true false false true true true
-                                  false)
-                               (String
-                                  (Ascii false false true true false true
-                                     true false)
-                                  (String
-                                     (Ascii false false true false false true
-                                        true false)
-                                     (String
-                                        (Ascii true false false false false
-                                           true false false) EmptyString))))))))))) in
-   substring 0
-     (findex 0
-        (String (Ascii false false false false false true false false)
-           EmptyString) v) v).
-
-
-
+Eval compute in "Hello".
+Eval compute in "".
+Eval compute in (fun x => String x "hello").
+Eval compute in "\".
+Eval compute in "A two-lines sentence that includes 
+	a tabulation and a beep".
+Eval compute in """".
+Eval compute in (let v := "Hello world!" in substring 0 (findex 0 " " v) v).
